WIP: Split and generalize compile dataflow tree

dataplane/Examples/Batch_op_Correctness.thy
@@ -18,9 +18,9 @@ abbreviation "t_1_0 \<equiv> MyPair (Suc 0) (0 :: nat)"
 abbreviation "t_0_1 \<equiv> MyPair (0 :: nat) (Suc 0)"
 abbreviation "t_1_1 \<equiv> MyPair (Suc 0) (Suc 0)"
 
-abbreviation "list_inps2 \<equiv> 
+abbreviation "list_inps_test \<equiv> 
  [Mint t_1_0, Mint t_0_1, Mint t_1_1, Drop t0, Data t_1_1 10, Drop t_1_1, Data t_0_1 7, Data t_1_0 (3 :: nat), Drop t_1_0, Drop t_0_1]"
-abbreviation "inps2 \<equiv> llist_of list_inps2"
+abbreviation "inps_test \<equiv> llist_of list_inps_test"
 
 abbreviation init_input_state where
 "init_input_state su inps \<equiv> \<lparr> 
@@ -38,8 +38,6 @@ abbreviation init_input_state where
    de1 = projl,
    es = inps
    \<rparr>"
-abbreviation "l1 inps \<equiv> Logic (ooo_input_op {|1|} (init_input_state default_internal_summary inps)) default_internal_summary"
-
 abbreviation init_operator_state_ty2 where
 "init_operator_state_ty2 su \<equiv> \<lparr> 
    summar = su,
@@ -57,11 +55,12 @@ abbreviation init_operator_state_ty2 where
    en2 = Inr,
    de2 = projr
    \<rparr>"
-abbreviation "l2 f \<equiv> Logic (batch_op (init_operator_state_ty2 default_internal_summary) f) default_internal_summary"
 
-abbreviation "test_dt2 \<equiv> Comp [(0, 1) \<mapsto> (0, 1)] (l1 (\<lambda> _. inps2)) (l2 (\<lambda> b. if b = [] then trace (STR ''Empty batch! ! !'') [] else [Max (set b)]))"
+abbreviation "l1 ip_state \<equiv> ((Logic (ooo_input_op {|1 :: 1|} ip_state) default_internal_summary) :: ('a, _, (_, 't) shared_state + (1 \<Rightarrow> 't antichain), 'c \<times> 't, 't :: {ccompare,canonically_ordered_monoid_add,ordered_ab_semigroup_monoid_add_imp_le,bot}) dataflow_tree)"
+abbreviation "l2 os2 f \<equiv> Logic (batch_op os2 f) default_internal_summary"
+abbreviation "G f ip_state os2 cbuf \<equiv> Comp [(0 :: 2, 1) \<mapsto> (0, 1)] cbuf (l1 (ip_state :: (1, 'd1 + 'd2, 'd1, _) input_state)) (l2 (os2 :: (1, 'd1 + 'd2, 'd1, 'd2, _) operator_state_ty2) f)"
 
-abbreviation "test_op \<equiv> compile_dataflow test_dt2 :: (2 \<times> 1, 2 \<times> 1, _) op"
+abbreviation "test_op \<equiv> compile_dataflow (G (\<lambda> b. if b = [] then trace (STR ''Empty batch! ! !'') [] else [Max (set b)]) (init_input_state default_internal_summary (\<lambda> _. inps_test)) (init_operator_state_ty2 default_internal_summary) (\<lambda> _. []) ) :: (2 \<times> 1, 2 \<times> 1, _) op"
 
 value [GHC] "lmap (\<lambda> io. case io of VOut p (x, t) \<Rightarrow> (projr x, t)) (trace_exec test_op)"
 value [GHC] "check_prefix 100 [((1, 1), (Inr 10, MyPair 1 1)), ((1, 1), (Inr 7, MyPair 0 1)),((1, 1), (Inr 3, MyPair 1 0))] test_op"
@@ -77,15 +76,18 @@ abbreviation "ts inps \<equiv> cimage (\<lambda> e. case e of Data t d \<Rightar
 abbreviation "inp_op os \<equiv> map_op (case_option (Inl (0 :: 2)) (\<lambda> p. Inr (0, p))) (case_option (Inl (0 :: 2)) (\<lambda> p. Inr (0, p))) (ooo_input_op {|1|} os)"
 abbreviation "tt_op os f \<equiv> map_op (case_option (Inl (1 :: 2)) (\<lambda> p. Inr (1, p))) (case_option (Inl (1 :: 2)) (\<lambda> p. Inr (1, p))) (batch_op os f)"
 
-abbreviation "G_op os1 cbuf os2 f \<equiv>
+abbreviation "G_op f ip_state os2 cbuf \<equiv>
+   dataflow_tree_to_operator (G f (ip_state :: (1, 'd1 + 'd2, 'd1, _) input_state) (os2 :: (1, 'd1 + 'd2, 'd1, 'd2, _) operator_state_ty2) cbuf)"
+
+(* abbreviation "G_op os1 cbuf os2 f \<equiv>
    map_op (case_sum id id) (case_sum id id)
    (comp_op [Inr (0 :: 2, 0 :: 1) \<mapsto> Inr (1 :: 2, 0 :: 1)] cbuf (inp_op (os1\<lparr> en1 := Inl \<rparr>)) (tt_op (os2\<lparr> de1 := projl, en2 := Inr \<rparr>) f))"
-
+ *)
 definition "c_pts_inv c caps = (\<forall> l. c_pts c l = caps l)"
 definition "Src_caps_inv caps oss = (\<forall> nid p. caps (Loc nid (Src p)) = zmset_of (mset (ocaps (oss nid) p)))"
 definition "Trg_caps_inv caps bufs = (\<forall> nid p. caps (Loc nid (Trg p)) = zmset_of (mset (map snd (bufs nid p))))"
 definition "extract_prog eds oss = concat (map (\<lambda> nid. extract_progress nid eds (snd (obtain_progress (oss nid)))) Enum.enum)"
-definition "front_inv oss c = (\<forall> nid p. front (oss nid) 1 \<le> frontier (c_imp c (Loc nid (Trg p))))"
+definition "front_inv oss c = (\<forall> nid p. front (oss nid) p \<le> frontier (c_imp c (Loc nid (Trg p))))"
 definition "imp_front_inv su c = (\<forall> l. frontier (c_imp c l) \<le> dataflow_topology.implied_frontier_alt su (+) c l)"
 definition "buf_imp_front_inv su c T nid p = (\<forall> t \<in> T. frontier_less_equal (dataflow_topology.implied_frontier_alt su (+) c (Loc nid (Trg p))) t)"
 definition "changes_above_impl_inv su c cgs = (\<forall>(l, t, d)\<in>set cgs. frontier_less_equal (dataflow_topology.implied_frontier_alt su (+) c l) t)"
@@ -104,7 +106,7 @@ lemma correctness_gen:
   assumes
     SUBGRAPH_INV:
     \<open>c = pt_tr sg\<close>
-    \<open>my_summ = summ sg\<close>
+    \<open>summ sg = dataflow_tree_to_graph (G f ip_state bt_state gbuf)\<close>
     \<open>edges sg = (\<lambda> l. if l = Loc 0 (Src 1) then [Loc 1 (Trg 1)] else [])\<close>
     and
     OP_STATE_INV: 
@@ -116,6 +118,7 @@ lemma correctness_gen:
     \<open>input (oss 2) 1 = map (\<lambda> (d, t). (Inl d, t)) inp_os2\<close>
     \<open>buf = out_os1 @ cbuf @ inp_os2\<close>
     \<open>bufs = (\<lambda> nid p. if nid = 1 \<and> p = 0 then buf else [])\<close>
+    \<open>gbuf = (\<lambda> p. case p of Inl x \<Rightarrow> [] | Inr x \<Rightarrow> map (\<lambda> (d, t). Inr (Inl d, t)) cbuf)\<close>
     and
     C_PTS_INV:
     \<open>Src_caps_inv caps oss\<close>
@@ -135,11 +138,8 @@ lemma correctness_gen:
     and
     PROP_INV:
     \<open>propagation_inv my_summ c\<close>
-
   shows 
-    \<open>set_op S D
-    (dataflow_op sg (G_op ip_state (\<lambda> p. case p of Inl x \<Rightarrow> [] | Inr x \<Rightarrow> map (\<lambda> (d, t). Inr (Inl d, t)) cbuf) bt_state f)) \<approx>
-    set_spec_op (cUn S S') D\<close>
+    \<open>set_op S D (dataflow_op sg (G_op f ip_state bt_state gbuf)) \<approx> set_spec_op (cUn S S') D\<close>
   oops
 
 
@@ -147,7 +147,7 @@ lemma correctness_gen:
 
 section \<open>Correctness\<close>
 
-abbreviation "G inps f \<equiv> compile_dataflow (Comp [(0, 1) \<mapsto> (0, 1)] (l1 inps) (l2 f))"
+(* abbreviation "G inps f \<equiv> compile_dataflow (Comp [(0, 1) \<mapsto> (0, 1)] (l1 inps) (l2 f))"
 
 lemma
   fixes inps :: \<open>1 \<Rightarrow> ('t :: {ccompare,canonically_ordered_monoid_add,ordered_ab_semigroup_monoid_add_imp_le,bot}, 'd1) event llist\<close>
@@ -156,6 +156,6 @@ lemma
  assumes \<open>S = cUnion (cimage (\<lambda> t. (cset_of_llist o llist_of) (map (\<lambda> x. ((2, 1), (Inr x, t))) (f (coll (inps 1) t)))) (ts (inps 1)))\<close>
   shows \<open>set_op {||} {||} (G inps f) \<approx> set_spec_op S {||}\<close>
   oops
-
+ *)
 
 end
